src/examples/seqs.v
@@ -1,0 +1,66 @@
+From iris.base_logic.lib Require Import invariants.
+From BurrowLang Require Import lang simp adequacy primitive_laws.
+From Tpcms Require Import rwlock.
+Require Import Burrow.tpcms.
+Require Import Burrow.ra.
+Require Import Burrow.rollup.
+Require Import Burrow.CpdtTactics.
+Require Import Burrow.tactics.
+
+From iris.base_logic Require Export base_logic.
+From iris.program_logic Require Export weakestpre.
+From iris.proofmode Require Import tactics.
+From iris.program_logic Require Import ectx_lifting.
+From BurrowLang Require Import notation tactics class_instances.
+From BurrowLang Require Import heap_ra.
+From BurrowLang Require Import lang.
+From iris Require Import options.
+
+(* really crummy sequence library *)
+
+Definition seq_idx : lang.expr :=
+  (rec: "seq_idx" "i" "array" :=
+      if: (BinOp EqOp "i" #0) then
+        Fst "array"
+      else
+        "seq_idx" ("i" + #(-1)) (Snd "array")
+  ).
+  
+Fixpoint has_elem (v: lang.val) (i: nat) : Prop :=
+  match i, v with
+  | O, (PairV l _ ) => True
+  | S i, (PairV _ r ) => has_elem r i
+  | _, _ => False
+  end.
+
+Fixpoint elem (v: lang.val) (i: nat) :=
+  match i, v with
+  | O, (PairV l _ ) => l
+  | S i, (PairV _ r ) => elem r i
+  | _, _ => #()
+  end.
+  
+Section SeqProof.
+
+Context `{!simpGS 𝜇 Σ}.
+
+Lemma wp_seq_idx (seq: lang.val) (i: nat)
+  (he: has_elem seq i) :
+      {{{ True }}}
+      seq_idx #i seq
+      {{{ RET (elem seq i); True }}}.
+Proof.
+  iIntros (P) "_ P". unfold seq_idx. wp_pures.
+  generalize he. generalize i. clear he. clear i. induction seq; intros i he.
+    - cbn [has_elem] in he. destruct i; contradiction.
+    - cbn [has_elem] in he. destruct i; contradiction.
+    - cbn [has_elem] in he. destruct i.
+      + wp_pures. unfold elem.
+        iModIntro. iApply "P". trivial.
+      + wp_pures.
+        replace ((Z.add (S i) (Zneg xH))) with (i : Z) by lia.
+        cbn [elem].
+        apply IHseq2; trivial.
+Qed.
+
+End SeqProof.
